\begin{enumerate}
    \item XOR Convolution
        \vspace{-1em}
        \begin{itemize}
            \itemsep-0.3em
            \item $f(A) = (f(A_0) + f(A_1), f(A_0) - f(A_1))$
            \item $f^{-1}(A) = (f^{-1}(\frac{A_0 + A_1}{2}), f^{-1}(\frac{A_0 - A_1}{2}))$
        \end{itemize}
    \item OR Convolution
        \vspace{-1em}
        \begin{itemize}
            \itemsep-0.3em
            \item $f(A) = (f(A_0), f(A_0) + f(A_1))$
            \item $f^{-1}(A) = (f^{-1}(A_0), f^{-1}(A_1) - f^{-1}(A_0))$
        \end{itemize}
    \item AND Convolution
        \vspace{-1em}
        \begin{itemize}
            \itemsep-0.3em
            \item $f(A) = (f(A_0) + f(A_1), f(A_1))$
            \item $f^{-1}(A) = (f^{-1}(A_0) - f^{-1}(A_1), f^{-1}(A_1))$
        \end{itemize}
\end{enumerate}
